proof/proof/ktcore_proof/sigpred.v
@@ -18,8 +18,7 @@ Collection W := sem.
 (** VRF sig. *)
 
 Definition vrfP γ (vrfPk : list w8) : iProp Σ :=
-  let γ' := γ.(AdtrAgree.agree) in
-  "%Heq_vrfPk" ∷ ⌜vrfPk = γ'.(Agree.vrf_pk)⌝.
+  "%Heq_vrfPk" ∷ ⌜vrfPk = γ.(Agree.vrf_pk)⌝.
 
 Definition vrfP_aux γ enc : iProp Σ :=
   ∃ vrfPk,
@@ -40,14 +39,13 @@ Qed.
 
 Definition linkP γ (ep : w64) link : iProp Σ :=
   ∃ digs,
-  let γ' := γ.(AdtrAgree.agree) in
-  "%Hinv" ∷ ⌜hashchain.valid digs γ.(AdtrAgree.cut)
+  "%Hinv" ∷ ⌜hashchain.valid digs γ.(Agree.cut)
     link (S $ uint.nat ep)⌝ ∗
-  "#Hlb_digs" ∷ mono_list_lb_own γ'.(Agree.digs) digs ∗
-  "%Hlen_digs" ∷ ⌜S $ uint.nat ep = (γ'.(Agree.digs_start) + length digs)%nat⌝ ∗
+  "#Hlb_digs" ∷ mono_list_lb_own γ.(Agree.digs) digs ∗
+  "%Hlen_digs" ∷ ⌜S $ uint.nat ep = (γ.(Agree.digs_start) + length digs)%nat⌝ ∗
   (* we started auditing at least by this epoch. *)
-  "%Hlt_audit" ∷ ⌜(γ'.(Agree.digs_start) + γ.(AdtrAgree.audit_start))%nat ≤ uint.nat ep⌝ ∗
-  "%Hmono_plain" ∷ ⌜mono_plain γ'.(Agree.vrf_pk) (drop γ.(AdtrAgree.audit_start) digs)⌝.
+  "%Hlt_audit" ∷ ⌜(γ.(Agree.digs_start) + γ.(Agree.func_start))%nat ≤ uint.nat ep⌝ ∗
+  "%Hmono_plain" ∷ ⌜mono_plain γ.(Agree.vrf_pk) (drop γ.(Agree.func_start) digs)⌝.
 
 Definition linkP_aux γ enc : iProp Σ :=
   ∃ ep link,
