proof/proof/server_proof/server.v
@@ -23,7 +23,7 @@ Record t :=
     pendγ : gname;
     (* map from uid to gname. *)
     uidγ : gmap w64 gname;
-    adtrγ : ktcore.AdtrAgree.t;
+    agreeγ : ktcore.Agree.t;
   }.
 End cfg.
 
@@ -51,7 +51,7 @@ Collection W := sem.
 instead of [into_sep_fractional_half] (priority 100).
 not sure if this is a bug in instance priority. *)
 Definition own_aux γ obj q : iProp Σ :=
-  let agreeγ := γ.(cfg.adtrγ).(ktcore.AdtrAgree.agree) in
+  let agreeγ := γ.(cfg.agreeγ) in
   "Hown_pend" ∷ dghost_var γ.(cfg.pendγ) (DfracOwn q) obj.(state.pending) ∗
   (* client remembers lb's of this. *)
   "Hown_hist" ∷ mono_list_auth_own agreeγ.(ktcore.Agree.digs) q obj.(state.hist).
@@ -102,7 +102,7 @@ Proof.
 Qed.
 
 Definition valid γ obj : iProp Σ :=
-  let agreeγ := γ.(cfg.adtrγ).(ktcore.AdtrAgree.agree) in
+  let agreeγ := γ.(cfg.agreeγ) in
   "#Hperm_uids" ∷ ([∗ map] uid ↦ pks ∈ obj.(state.pending),
     ∃ uidγ,
     "%Hlook_uidγ" ∷ ⌜γ.(cfg.uidγ) !! uid = Some uidγ⌝ ∗
@@ -128,7 +128,7 @@ Definition is_inv γ := inv nroot (∃ obj, inv_aux γ obj).
 (** helpers for inv. *)
 
 Lemma hist_pks_prefix uid γ (i j : nat) (x y : list w8) :
-  let agreeγ := γ.(cfg.adtrγ).(ktcore.AdtrAgree.agree) in
+  let agreeγ := γ.(cfg.agreeγ) in
   (i ≤ j)%nat →
   is_inv γ -∗
   mono_list_idx_own agreeγ.(ktcore.Agree.digs) i x -∗
@@ -148,7 +148,7 @@ Proof.
 Qed.
 
 Lemma hist_to_put_perms γ i x :
-  let agreeγ := γ.(cfg.adtrγ).(ktcore.AdtrAgree.agree) in
+  let agreeγ := γ.(cfg.agreeγ) in
   is_inv γ -∗
   mono_list_idx_own agreeγ.(ktcore.Agree.digs) i x ={⊤}=∗
   ∀ uid pks,
@@ -203,12 +203,12 @@ Definition perm_read γ Q : iProp Σ :=
         ={∅,⊤}=∗ Q obj)).
 
 Definition Q_read_lb prev_lb γ obj : iProp Σ :=
-  let agreeγ := γ.(cfg.adtrγ).(ktcore.AdtrAgree.agree) in
+  let agreeγ := γ.(cfg.agreeγ) in
   mono_list_lb_own agreeγ.(ktcore.Agree.digs) obj.(state.hist) ∗
   ⌜prev_lb `prefix_of` obj.(state.hist)⌝.
 
 Lemma op_read_lb γ prev_lb :
-  let agreeγ := γ.(cfg.adtrγ).(ktcore.AdtrAgree.agree) in
+  let agreeγ := γ.(cfg.agreeγ) in
   is_inv γ -∗
   mono_list_lb_own agreeγ.(ktcore.Agree.digs) prev_lb -∗
   perm_read γ (Q_read_lb prev_lb γ).
@@ -230,7 +230,7 @@ Proof.
 Qed.
 
 Definition Q_read_idx prev_idx γ obj : iProp Σ :=
-  let agreeγ := γ.(cfg.adtrγ).(ktcore.AdtrAgree.agree) in
+  let agreeγ := γ.(cfg.agreeγ) in
   mono_list_lb_own agreeγ.(ktcore.Agree.digs) obj.(state.hist) ∗
   ⌜prev_idx < length obj.(state.hist)⌝.
 
@@ -240,7 +240,7 @@ at currying time, not under good flag, so client doesn't have prev_lb.
 but it does have have prev_idx!
 that's an arg to, e.g., CallHistory, independent of good-ness. *)
 Lemma op_read_idx γ prev_idx (a : list w8) :
-  let agreeγ := γ.(cfg.adtrγ).(ktcore.AdtrAgree.agree) in
+  let agreeγ := γ.(cfg.agreeγ) in
   is_inv γ -∗
   mono_list_idx_own agreeγ.(ktcore.Agree.digs) prev_idx a -∗
   perm_read γ (Q_read_idx prev_idx γ).
@@ -309,7 +309,7 @@ Proof.
 Qed.
 
 Definition perm_add_hist γ : iProp Σ :=
-  let agreeγ := γ.(cfg.adtrγ).(ktcore.AdtrAgree.agree) in
+  let agreeγ := γ.(cfg.agreeγ) in
   □ (|={⊤,∅}=> ∃ obj, own γ obj ∗
     ∀ dig,
     ⌜ktcore.to_plain agreeγ.(ktcore.Agree.vrf_pk) dig = obj.(state.pending)⌝ -∗
@@ -367,12 +367,11 @@ Collection W := sem.
 #[local] Set Default Proof Using "W".
 
 Definition own γ ptr obj : iProp Σ :=
-  let adtrγ := γ.(cfg.adtrγ) in
-  let agreeγ := adtrγ.(ktcore.AdtrAgree.agree) in
+  let agreeγ := γ.(cfg.agreeγ) in
   ∃ ptr_sig ptr_vrf sl_commit,
   "#Hstr_secrets" ∷ ptr ↦□ (server.secrets.mk ptr_sig ptr_vrf sl_commit) ∗
   "#Hown_sig" ∷ cryptoffi.own_sig_sk ptr_sig γ.(cfg.sig_pk)
-    (sigpred.P adtrγ) ∗
+    (sigpred.P agreeγ) ∗
   "#Hown_vrf" ∷ cryptoffi.own_vrf_sk ptr_vrf agreeγ.(ktcore.Agree.vrf_pk) ∗
   "#Hsl_commit" ∷ sl_commit ↦*□ obj.(commit) ∗
   "%Hlen_commit" ∷ ⌜Z.of_nat (length obj.(commit)) = cryptoffi.hash_len⌝.
@@ -404,7 +403,7 @@ Definition is_commit commit_sec (hidden : gmap (list w8) (list w8)) :=
     hidden.
 
 Definition own γ ptr secs dig q : iProp Σ :=
-  let agreeγ := γ.(cfg.adtrγ).(ktcore.AdtrAgree.agree) in
+  let agreeγ := γ.(cfg.agreeγ) in
   ∃ ptr_hidden hidden ptr_plain ptr0_plain,
   let plain := ktcore.to_plain agreeγ.(ktcore.Agree.vrf_pk) dig in
   "#Hstr_keyStore" ∷ ptr ↦□ (server.keyStore.mk ptr_hidden ptr_plain) ∗
@@ -438,7 +437,7 @@ Definition is_audits γ digs audits : iProp Σ :=
     "#His_sig" ∷ ktcore.wish_LinkSig γ.(cfg.sig_pk) (W64 ep) link aud.(ktcore.AuditProof.LinkSig)).
 
 Definition own γ ptr digs q : iProp Σ :=
-  let agreeγ := γ.(cfg.adtrγ).(ktcore.AdtrAgree.agree) in
+  let agreeγ := γ.(cfg.agreeγ) in
   ∃ ptr_chain sl_audits sl0_audits audits sl_vrfSig vrfSig,
   "Hstr_history" ∷ ptr ↦{#q} (server.history.mk ptr_chain sl_audits sl_vrfSig) ∗
   "Hown_chain" ∷ hashchain.own ptr_chain digs (DfracOwn q) ∗
@@ -512,7 +511,7 @@ Collection W := sem.
 #[local] Set Default Proof Using "W".
 
 Definition own γ secs ptr obj : iProp Σ :=
-  let agreeγ := γ.(cfg.adtrγ).(ktcore.AdtrAgree.agree) in
+  let agreeγ := γ.(cfg.agreeγ) in
   ∃ sl_pk sl_mapLabel mapLabel sl_mapVal mapVal rand,
   "#Hstr_work" ∷ ptr ↦□ (server.work.mk obj.(uid) obj.(ver) sl_pk sl_mapLabel sl_mapVal) ∗
   "#Hsl_pk" ∷ sl_pk ↦*□ obj.(pk) ∗
@@ -559,8 +558,7 @@ Definition own_ro γ ptr obj : iProp Σ :=
   "#His_workQ" ∷ bag.is_chan_bag workQγ ptr_workQ (work.own_aux γ obj.(secs)).
 
 Definition own γ ptr σ obj q : iProp Σ :=
-  let adtrγ := γ.(cfg.adtrγ) in
-  let agreeγ := adtrγ.(ktcore.AdtrAgree.agree) in
+  let agreeγ := γ.(cfg.agreeγ) in
   ∃ ptr_keys ptr_hist last_dig,
   "#Hfld_keys" ∷ ptr.[server.Server.t, "keys"] ↦□ ptr_keys ∗
   "#Hfld_hist" ∷ ptr.[server.Server.t, "hist"] ↦□ ptr_hist ∗
@@ -574,8 +572,8 @@ Definition own γ ptr σ obj q : iProp Σ :=
   "%Heq_hist_pend" ∷ ⌜ktcore.to_plain agreeγ.(ktcore.Agree.vrf_pk) last_dig = σ.(state.pending)⌝ ∗
   "#Hperm_add_hist" ∷ perm_add_hist γ ∗
   "%Heq_digs_start" ∷ ⌜agreeγ.(ktcore.Agree.digs_start) = 0%nat⌝ ∗
-  "%Heq_cut" ∷ ⌜adtrγ.(ktcore.AdtrAgree.cut) = None⌝ ∗
-  "%Heq_audit_start" ∷ ⌜adtrγ.(ktcore.AdtrAgree.audit_start) = 0%nat⌝.
+  "%Heq_cut" ∷ ⌜agreeγ.(ktcore.Agree.cut) = None⌝ ∗
+  "%Heq_audit_start" ∷ ⌜agreeγ.(ktcore.Agree.func_start) = 0%nat⌝.
 
 Definition own_aux γ ptr obj q : iProp Σ := ∃ σ, own γ ptr σ obj q.
 
@@ -598,7 +596,7 @@ Collection W := sem + package_sem.
 (** fetch-side helper funcs. *)
 
 Lemma wp_Server_getHist s γ σ obj (uid prefixLen : w64) q last_dig :
-  let agreeγ := γ.(cfg.adtrγ).(ktcore.AdtrAgree.agree) in
+  let agreeγ := γ.(cfg.agreeγ) in
   let pks := ktcore.to_pks agreeγ.(ktcore.Agree.vrf_pk) uid last_dig in
   {{{
     is_pkg_init server ∗
@@ -625,7 +623,7 @@ Proof.
   simplify_eq/=. wp_auto.
   wp_apply (wp_map_lookup1 with "[$Hptr_plain]") as "Hptr_plain".
   (* destruct "uid existence" early to reduce complexity. *)
-  destruct (ktcore.to_plain (γ.(cfg.adtrγ).(ktcore.AdtrAgree.agree).(ktcore.Agree.vrf_pk)) last_dig !! uid) as [pks|] eqn:Hlook_uid.
+  destruct (ktcore.to_plain (γ.(cfg.agreeγ).(ktcore.Agree.vrf_pk)) last_dig !! uid) as [pks|] eqn:Hlook_uid.
   2: {
     rewrite lookup_total_alt Hlook_uid /= in Heq_prefixLen |-*.
     iDestruct (big_sepM2_lookup_r_none with "Hptr0_plain") as %->; [done|].
@@ -661,7 +659,7 @@ Proof.
     "Hcap_hist" ∷ own_slice_cap loc sl_hist 1 ∗
     "#Hsl0_hist" ∷ ([∗ list] ptr;obj ∈ sl0_hist;hist, ktcore.Memb.own ptr obj (□)) ∗
 
-    "#Hwish_hist" ∷ ktcore.wish_ListMemb (γ.(cfg.adtrγ).(ktcore.AdtrAgree.agree).(ktcore.Agree.vrf_pk)) uid
+    "#Hwish_hist" ∷ ktcore.wish_ListMemb (γ.(cfg.agreeγ).(ktcore.Agree.vrf_pk)) uid
       (uint.nat prefixLen) last_dig hist ∗
     "%Heq_hist" ∷ ⌜subslice (uint.nat prefixLen) (uint.nat ver) pks =
       ktcore.CommitOpen.Val <$> (ktcore.Memb.PkOpen <$> hist)⌝
@@ -741,7 +739,7 @@ Proof.
 Qed.
 
 Lemma wp_Server_getBound s γ σ obj (uid numVers : w64) q last_dig :
-  let agreeγ := γ.(cfg.adtrγ).(ktcore.AdtrAgree.agree) in
+  let agreeγ := γ.(cfg.agreeγ) in
   let pks := ktcore.to_pks agreeγ.(ktcore.Agree.vrf_pk) uid last_dig in
   {{{
     is_pkg_init server ∗
@@ -837,7 +835,7 @@ Proof.
 
   iAssert (
     ∃ (i : w64) (t0 : loc) sl_upd sl0_upd upd new_dig,
-    let agreeγ := γ.(cfg.adtrγ).(ktcore.AdtrAgree.agree) in
+    let agreeγ := γ.(cfg.agreeγ) in
     let new_pend := ktcore.to_plain agreeγ.(ktcore.Agree.vrf_pk) new_dig in
     "i" ∷ i_ptr ↦ i ∗
     "%Hlt_i" ∷ ⌜0 ≤ sint.Z i ≤ length work⌝ ∗
@@ -879,7 +877,7 @@ Proof.
     (* unify cases of uid in or not in golang map. *)
     iAssert (
       ∃ sl0_pks,
-      let agreeγ := γ.(cfg.adtrγ).(ktcore.AdtrAgree.agree) in
+      let agreeγ := γ.(cfg.agreeγ) in
       let sl_pks := default slice.nil (ptr0_plain !! w.(work.uid)) in
       "Hsl_pks" ∷ sl_pks ↦* sl0_pks ∗
       "Hcap_pks" ∷ own_slice_cap slice.t sl_pks 1 ∗
@@ -903,7 +901,7 @@ Proof.
     iDestruct (own_slice_len with "Hsl_pks") as %?.
     iDestruct (big_sepL2_length with "Hsl0_pks") as %?.
 
-    iAssert (let agreeγ := γ.(cfg.adtrγ).(ktcore.AdtrAgree.agree) in
+    iAssert (let agreeγ := γ.(cfg.agreeγ) in
       ⌜uint.nat w.(work.ver) =
       length $ ktcore.to_pks agreeγ.(ktcore.Agree.vrf_pk) w.(work.uid) old_dig⌝)%I
       as %Heq_ver; [word|].
@@ -971,7 +969,7 @@ Proof.
     - instantiate (1:=ktcore.UpdateProof.mk' _ _ _). iFrame "#".
     - done.
     - by iApply ktcore.wish_ListUpdate_grow.
-    - trans (ktcore.to_plain (γ.(cfg.adtrγ).(ktcore.AdtrAgree.agree).(ktcore.Agree.vrf_pk)) old_dig); [done|].
+    - trans (ktcore.to_plain (γ.(cfg.agreeγ).(ktcore.Agree.vrf_pk)) old_dig); [done|].
       apply insert_included; [apply _|].
       intros.
       setoid_rewrite lookup_total_correct; [|done].
@@ -1008,7 +1006,7 @@ Proof.
 
   iDestruct (own_slice_len with "Hsl_audits") as %?.
   iDestruct (big_sepL2_length with "Hown_audits") as %?.
-  eassert (ktcore.mono_plain (γ.(cfg.adtrγ).(ktcore.AdtrAgree.agree).(ktcore.Agree.vrf_pk)) (_ ++ [_])) as Hmono_plain'.
+  eassert (ktcore.mono_plain (γ.(cfg.agreeγ).(ktcore.Agree.vrf_pk)) (_ ++ [_])) as Hmono_plain'.
   { rewrite /ktcore.mono_plain in Hmono_plain |-*.
     rewrite !fmap_app.
     eapply list_reln_snoc; [done|].
@@ -1101,7 +1099,7 @@ Lemma wp_Server_History s γ obj (uid prevEpoch prevVerLen : w64) Q :
   {{{
     sl_chainProof sl_linkSig sl_hist ptr_bound err σ lastDig,
     RET (#sl_chainProof, #sl_linkSig, #sl_hist, #ptr_bound, #err);
-    let agreeγ := γ.(cfg.adtrγ).(ktcore.AdtrAgree.agree) in
+    let agreeγ := γ.(cfg.agreeγ) in
     let numEps := length σ.(state.hist) in
     let pks := ktcore.to_pks agreeγ.(ktcore.Agree.vrf_pk) uid lastDig in
     "Hown_serv_lock" ∷ Server.lock_perm γ s obj ∗
@@ -1163,7 +1161,7 @@ Proof.
     wp_end. iFrame "∗#%". word. }
   simpl.
   wp_apply (wp_map_lookup1 with "[$Hptr_plain]") as "Hptr_plain".
-  iAssert (let agreeγ := γ.(cfg.adtrγ).(ktcore.AdtrAgree.agree) in
+  iAssert (let agreeγ := γ.(cfg.agreeγ) in
     ⌜sint.Z (default slice.nil (ptr0_plain !! uid)).(slice.len) =
     length $ ktcore.to_pks agreeγ.(ktcore.Agree.vrf_pk) uid last_dig⌝)%I as %?.
   { rewrite /keyStore.own_plain.
@@ -1312,7 +1310,7 @@ Lemma wp_Server_Start s γ obj Q :
   s @! (go.PointerType server.Server) @! "Start" #()
   {{{
     chain vrf ptr_chain ptr_vrf σ last_link, RET (#ptr_chain, #ptr_vrf);
-    let agreeγ := γ.(cfg.adtrγ).(ktcore.AdtrAgree.agree) in
+    let agreeγ := γ.(cfg.agreeγ) in
     let numEps := length σ.(state.hist) in
     "Hown_serv_lock" ∷ Server.lock_perm γ s obj ∗
     "HQ" ∷ Q σ ∗
@@ -1402,15 +1400,15 @@ Lemma wp_New (uidγ : gmap w64 gname) :
     "Hlocks" ∷ ([∗] replicate (pred $ Z.to_nat rwmutex.actualMaxReaders)
       (Server.lock_perm γ ptr_server obj)) ∗
     "#Hsl_sigPk" ∷ sl_sigPk ↦*□ γ.(cfg.sig_pk) ∗
-    "#His_sigPk" ∷ cryptoffi.is_sig_pk γ.(cfg.sig_pk) (sigpred.P γ.(cfg.adtrγ))
+    "#His_sigPk" ∷ cryptoffi.is_sig_pk γ.(cfg.sig_pk) (sigpred.P γ.(cfg.agreeγ))
   }}}.
 Proof.
   wp_start as "@". wp_auto.
   wp_apply wp_alloc as "* Hptr_mu".
   wp_apply cryptoffi.wp_VrfGenerateKey as "* @".
   iMod (mono_list_own_alloc []) as (digsγ) "[Hauth_digs _]".
-  remember (ktcore.AdtrAgree.mk (ktcore.Agree.mk vrfPk digsγ 0%nat) None 0%nat) as adtrγ.
-  wp_apply (cryptoffi.wp_SigGenerateKey (sigpred.P adtrγ)) as "* @".
+  remember (ktcore.Agree.mk vrfPk digsγ 0%nat None 0%nat) as agreeγ.
+  wp_apply (cryptoffi.wp_SigGenerateKey (sigpred.P agreeγ)) as "* @".
   wp_apply cryptoffi.wp_VrfPrivateKey_PublicKey as "* @".
   { iFrame "#". }
   iRename "Hsl_enc" into "Hsl_vrfPk". iPersist "Hsl_vrfPk".
@@ -1455,7 +1453,7 @@ Proof.
 
   iMod (dghost_var_alloc (∅ : ktcore.plain_ty)) as (pendγ) "[Hgs_pend Hgs_pend']".
   eremember (Server.mk' (secrets.mk' commit_sec)) as obj.
-  eremember (cfg.mk sigPk pendγ uidγ adtrγ) as γ.
+  eremember (cfg.mk sigPk pendγ uidγ agreeγ) as γ.
   eremember (state.mk ∅ [hash]) as σ.
   iMod (start_bag (work.own_aux γ obj.(Server.secs)) with "His_chan Hown_chan")
     as "#His_chan_bag"; [done|].
